Proved something...

proof/SimModSem.v
@@ -17,6 +17,7 @@ Import ModSem.
 Require Import ModSemProps.
 Require Import Events.
 Require Import SmallstepC.
+From Paco Require Import hpattern.
 
 Set Implicit Arguments.
 
@@ -590,6 +591,33 @@ Qed.
 Inductive good_properties SM {SS: SimSymb.class SM}
           (SMOS: SimMemOhs.class) (msp: ModSemPair.t): Prop :=
 | good_properties_intro
+    (SMPROJ: forall smos (MWF: SimMemOhs.wf smos),
+        exists smo, sm_match msp smo smos /\ SimMemOh.wf smo)
+    (SMSIM: forall (smos0: SimMemOhs.t)
+                   (smo0 smo1: SimMemOh.t)
+                   (LE: SimMemOh.le smo0 smo1)
+                   (SMMATCH: sm_match msp smo0 smos0)
+                   (WFWF: SimMemOh.wf smo0 -> SimMemOhs.wf smos0)
+      ,
+        exists smos1, (<<SMSTEPBIG: SimMemOhs.le smos0 smos1>>)
+                      /\ (<<SMMATCH: sm_match msp smo1 smos1>>)
+                      /\ (<<WFWF: SimMemOh.wf smo1 -> SimMemOhs.wf smos1>>))
+    (SMSIMPRIV: forall (smos0: SimMemOhs.t)
+                       (smo0 smo1: SimMemOh.t)
+                       (SMMATCH: sm_match msp smo0 smos0)
+                       (LE: SimMemOh.lepriv smo0 smo1)
+                       (WFWF: SimMemOh.wf smo0 -> SimMemOhs.wf smos0)
+      ,
+        exists smos1, (<<SMSTEPBIG: SimMemOhs.lepriv smos0 smos1>>)
+                      /\ (<<SMMATCH: sm_match msp smo1 smos1>>)
+                      /\ (<<WFWF: SimMemOh.wf smo1 -> SimMemOhs.wf smos1>>))
+    (SMMATCHLE: forall smo0 smo1 smos0 smos1
+                       (SMMATCH0: sm_match msp smo0 smos0)
+                       (SMMATCH1: sm_match msp smo1 smos1)
+                       (SMLE: SimMemOhs.le smos0 smos1)
+      ,
+        <<SMLE: SimMemOh.le smo0 smo1>>
+    )
 .
 
 
@@ -605,26 +633,496 @@ Section SimMemOhsIntro.
       let name := fresh "let" in destruct x eqn:name
     end.
 
-  Definition o_get A (oa: option A) (default: A): A :=
-    match oa with
-    | Some a => a
-    | _ => default
+  Inductive SimMemOhs_t_aux: Midx.t -> Type :=
+  | TyNil: SimMemOhs_t_aux 0%nat
+  | TyCons
+      n msp
+      (MSP: List.nth_error msps n = Some msp)
+      (hd: (@SimMemOh.t _ _ _ msp.(ModSemPair.SMO)))
+      (tl: SimMemOhs_t_aux n)
+    :
+      SimMemOhs_t_aux (S n)
+  .
+
+  (* TODO: change to Let *)
+  Definition SimMemOhs_t: Type := SimMem.t * SimMemOhs_t_aux (length msps).
+
+  Inductive SimMemOhs_le_aux:
+    forall (midx: Midx.t) (smos0 smos1: SimMemOhs_t_aux midx), Prop :=
+  | LeNil smos0 smos1: @SimMemOhs_le_aux (0%nat) smos0 smos1
+  | LeCons
+      n msp
+      (MSP: List.nth_error msps n = Some msp)
+      (hd0 hd1: (@SimMemOh.t _ _ _ msp.(ModSemPair.SMO)))
+      (tl0 tl1: SimMemOhs_t_aux n)
+    :
+      @SimMemOhs_le_aux (S n) (@TyCons n msp MSP hd0 tl0)
+                        (@TyCons n msp MSP hd0 tl0)
+  .
+
+  (* TODO: change to Let *)
+  Definition SimMemOhs_le: SimMemOhs_t -> SimMemOhs_t -> Prop :=
+    fun smos0 smos1 =>
+      SimMem.le (fst smos0) (fst smos1) /\
+      @SimMemOhs_le_aux (length msps) (snd smos0) (snd smos1).
+
+  Program Instance PreOrder_SimMemOhs_le_aux: PreOrder SimMemOhs_le.
+  Next Obligation.
+    ii. rr. split; try refl. abstr (snd x) y.
+    induction y; ii; ss.
+    - econs.
+    - econs; eauto.
+  Qed.
+  Next Obligation.
+    unfold SimMemOhs_le.
+    ii. des. split; try etrans; eauto. clear H H0.
+    abstr (snd x) a. abstr (snd y) b. abstr (snd z) c.
+    ginduction a; ii; ss.
+    - inv H2. simpl_depind. clarify. econs.
+    - inv H2. simpl_depind. clarify. inv H1. simpl_depind. clarify.
+      replace MSP2 with MSP.
+      { econs; eauto. }
+      eapply Axioms.proof_irr.
+  Qed.
+
+  Inductive SimMemOhs_wf_aux (sm: SimMem.t):
+    forall (midx: Midx.t) (smos: SimMemOhs_t_aux midx), Prop :=
+  | WfNil smos: @SimMemOhs_wf_aux sm 0%nat smos
+  | WfCons
+      n msp
+      (MSP: List.nth_error msps n = Some msp)
+      (hd: (@SimMemOh.t _ _ _ msp.(ModSemPair.SMO)))
+      (tl: @SimMemOhs_t_aux n)
+      (HDEQ: hd.(SimMemOh.sm) = sm)
+      (HD: SimMemOh.wf hd)
+      (TL: @SimMemOhs_wf_aux sm n tl)
+    :
+      @SimMemOhs_wf_aux sm (S n) (@TyCons n msp MSP hd tl)
+  .
+
+  (* TODO: change to Let *)
+  Definition SimMemOhs_wf: SimMemOhs_t -> Prop :=
+    fun smos => SimMem.wf (fst smos)
+                /\ @SimMemOhs_wf_aux (fst smos) (length msps) (snd smos).
+
+  (* Let SimMemOhs_t: Type := *)
+  (*   SimMem.t * *)
+  (*   (forall midx, *)
+  (*       match List.nth_error msps midx with *)
+  (*       | Some msp => (@SimMemOh.t _ _ _ msp.(ModSemPair.SMO)) *)
+  (*       | None => SimMemOh.t *)
+  (*       end *)
+  (*   ). *)
+           
+  Fail Inductive SimMemOhs_ohs_src_aux:
+    forall (midx: Midx.t) (smos: SimMemOhs_t_aux midx), list { oh: Type & oh } :=
+  | OhsSrcNil smos: @SimMemOhs_ohs_src_aux 0%nat smos
+  .
+
+  Fixpoint SimMemOhs_ohs_src_aux2 (midx: Midx.t) (smos: SimMemOhs_t_aux midx):
+    list { oh: Type & oh } :=
+    match smos with
+    | TyNil => nil
+    | TyCons n msp MSP hd tl =>
+      (* (@existT Type _ _ hd) *)
+      (existT id _ hd.(SimMemOh.oh_src)) :: @SimMemOhs_ohs_src_aux2 n tl
     end
   .
 
-  Let SimMemOhs_t: Type :=
-    SimMem.t *
-    (forall midx,
-        match List.nth_error msps midx with
-        | Some msp => (@SimMemOh.t _ _ _ msp.(ModSemPair.SMO))
-        | None => SimMemOh.t
-        end
-        (* o_get (o_map (List.nth_error msps midx) *)
-        (*                   (fun msp => (@SimMemOh.t _ _ _ msp.(ModSemPair.SMO)))) *)
-        (*            SimMemOh.t *)
-    ).
+  (* TODO: make it Let *)
+  Definition SimMemOhs_ohs_src_aux: forall midx, SimMemOhs_t_aux midx -> Sem.Ohs :=
+    fun midx smos_aux n =>
+      match nth_error (rev (@SimMemOhs_ohs_src_aux2 midx smos_aux)) n with
+      | Some oh_src => oh_src
+      | _ => (existT id _ tt)
+      end
+  .
 
-  (* Ltac uo := CoqlibC.uo; unfold o_get in *. *)
+  (* TODO: make it Let *)
+  Definition SimMemOhs_ohs_src: SimMemOhs_t -> Sem.Ohs :=
+    fun smos => @SimMemOhs_ohs_src_aux (length msps) (snd smos)
+  .
+  (* Let SimMemOhs_ohs_src: SimMemOhs_t -> Sem.Ohs := *)
+  (*   fun smos midx => *)
+  (*     match nth_error (@SimMemOhs_ohs_src_aux (length msps) (snd smos)) midx with *)
+  (*     | Some oh_src => oh_src *)
+  (*     | _ => (existT id _ tt) *)
+  (*     end *)
+  (* . *)
+
+Record sm_match_tmp_aux (msp: @ModSemPair.t SM SS)
+  (smo: (@SimMemOh.t _ _ _ msp.(ModSemPair.SMO))) m (smos: SimMemOhs_t_aux m): Prop :=
+  (* TODO: I want to remove @ *)
+  {
+    ohsrcty_tmp: (projT1 ((@SimMemOhs_ohs_src_aux m smos) (msp.(ModSemPair.src).(midx)))) =
+             msp.(ModSemPair.src).(owned_heap);
+    ohsrc_tmp: (projT2 ((@SimMemOhs_ohs_src_aux m smos) (msp.(ModSemPair.src).(midx)))
+                   ~= smo.(SimMemOh.oh_src));
+  }.
+
+Definition sm_match_tmp (msp: @ModSemPair.t SM SS)
+  (smo: (@SimMemOh.t _ _ _ msp.(ModSemPair.SMO))) (smos: SimMemOhs_t): Prop :=
+  @sm_match_tmp_aux msp smo (length msps) (snd smos) /\ fst smos = smo.
+
+  (* Fixpoint get_nth (midx: Midx.t) (smos: SimMemOhs_t_aux midx) *)
+  (*          (n: Midx.t) msp (MSP: List.nth_error msps n = Some msp): *)
+  (*   (@SimMemOh.t _ _ _ msp.(ModSemPair.SMO)) := *)
+  (*   match smos with *)
+  (*   | TyNil => nil *)
+  (*   | TyCons n msp MSP hd tl => *)
+  (*     nil *)
+  (*   end *)
+  (* . *)
+
+End SimMemOhsIntro.
+Arguments sm_match_tmp {_ _}.
+Arguments sm_match_tmp_aux {_ _}.
+Arguments SimMemOhs_t {_ _}.
+Arguments SimMemOhs_wf {_ _}.
+Arguments SimMemOhs_wf_aux {_ _}.
+Arguments SimMemOh.t {_}.
+(* Arguments sm_match_tmp: clear implicits. *)
+
+  (* Goal forall `{SM: SimMem.class} {SS: SimSymb.class SM} *)
+  (*             (msps: list ModSemPair.t) *)
+  (*             len n (LT: (len > n)%nat) msp *)
+  (*             (MSP: nth_error msps n = Some msp), *)
+  (*     (<<SMPROJ: forall sm (smos: SimMemOhs_t_aux msps len) *)
+  (*                       (MWF0: SimMem.wf sm) *)
+  (*                       (MWF1: SimMemOhs_wf_aux msps sm len smos), *)
+  (*         exists (smo: (@SimMemOh.t _ _ _ msp.(ModSemPair.SMO))), *)
+  (*           sm = smo /\ *)
+  (*           (projT1 ((SimMemOhs_ohs_src_aux smos) *)
+  (*                      (msp.(ModSemPair.src).(midx)))) = *)
+  (*            msp.(ModSemPair.src).(owned_heap) /\ *)
+  (*           (projT2 ((SimMemOhs_ohs_src_aux smos) *)
+  (*                      (msp.(ModSemPair.src).(midx))) *)
+  (*                  ~= smo.(SimMemOh.oh_src)) /\ *)
+  (*           (* sm_match_tmp msps msp smo (sm, smos) /\ *) *)
+  (*           SimMemOh.wf smo>>). *)
+  (* Proof. *)
+  (*   (* intros ? ? ?. *) *)
+  (*   (* ginduction len; ii; ss. *) *)
+  (*   ii. gen n. *)
+  (*   dependent induction smos; ii; ss. *)
+  (*   { omega. } *)
+  (*   destruct n0; ss. *)
+  (*   { destruct msps; ss. clarify. *)
+  (*     exists hd. *)
+  (* hd : @SimMemOh.t SM (owned_heap (@ModSemPair.src SM SS msp0)) *)
+  (*        (owned_heap (@ModSemPair.tgt SM SS msp0)) msp0 *)
+  (*   smo : @SimMemOh.t SM (owned_heap (@ModSemPair.src SM SS msp)) *)
+  (*           (owned_heap (@ModSemPair.tgt SM SS msp)) msp, *)
+  (*   } *)
+  (* Qed. *)
+
+  Goal forall `{SM: SimMem.class} {SS: SimSymb.class SM}
+              (msps: list ModSemPair.t)
+              n msp
+              (MSP: nth_error msps n = Some msp),
+      (<<SMPROJ: forall (smos: SimMemOhs_t_aux msps (length msps)),
+          exists smo: (@SimMemOh.t _ _ _ msp.(ModSemPair.SMO)), True>>).
+  Proof.
+    ii.
+    assert((n < length msps)%nat).
+    { eapply nth_error_Some; eauto. rewrite MSP; ss. }
+    abstr (length msps) m. gen n.
+    dependent induction smos; ii; ss.
+    { omega. }
+    destruct (classic (n0 = n)).
+    { clarify. }
+    eapply IHsmos; eauto.
+    omega.
+  Qed.
+
+  Goal forall `{SM: SimMem.class} {SS: SimSymb.class SM}
+              (msps: list ModSemPair.t)
+              n msp
+              (MSP: nth_error msps n = Some msp),
+      (<<SMPROJ: forall smos (MWF: SimMemOhs_wf msps smos),
+          exists smo, sm_match_tmp msps msp smo smos /\ SimMemOh.wf smo>>).
+  Proof.
+    ii.
+    destruct smos as [sm smos].
+    assert((n < length msps)%nat).
+    { eapply nth_error_Some; eauto. rewrite MSP; ss. }
+    rr in MWF. des. ss.
+    (* Set Printing Implicit. *)
+    pattern (length msps) in smos.
+    Fail remember (length msps).
+    Fail generalize (length msps).
+  Abort.
+
+  Goal forall `{SM: SimMem.class} {SS: SimSymb.class SM}
+              (msps: list ModSemPair.t)
+              n msp
+              (MSP: nth_error msps n = Some msp),
+      (<<SMPROJ: forall smos (MWF: SimMemOhs_wf msps smos),
+          exists smo, sm_match_tmp_aux msps msp smo (length msps) (snd smos)
+                      /\ SimMemOh.sm smo = fst smos
+                      /\ SimMemOh.wf smo>>).
+  Proof.
+    ii.
+    assert((n < length msps)%nat).
+    { eapply nth_error_Some; eauto. rewrite MSP; ss. }
+    destruct smos as [sm smos]; ss.
+    gen smos.
+    Fail generalize (length msps).
+  Abort.
+
+  Goal forall `{SM: SimMem.class} {SS: SimSymb.class SM}
+              (msps: list ModSemPair.t)
+              n msp
+              (MSP: nth_error msps n = Some msp),
+      (<<SMPROJ: forall (smos: SimMemOhs_t msps), exists smo, fst smos = smo>>).
+  Proof.
+    ii.
+    gen n.
+    destruct smos as [sm smos].
+    dependent induction smos; ii; ss.
+    { destruct msps; ss. clarify. destruct n; ss. }
+    destruct msps; ss. clarify.
+    dependent destruction smos0.
+    simpl_depind. clarify. simpl_depind. clarify.
+    idtac "IHsmos-is-not well-formed".
+  Abort.
+
+  Lemma ohs_src_aux2_length
+        `{SM: SimMem.class} {SS: SimSymb.class SM}
+        (msps: list ModSemPair.t)
+        m (smos: SimMemOhs_t_aux msps m)
+    :
+      length (SimMemOhs_ohs_src_aux2 smos) = m
+  .
+  Proof.
+    ginduction m; ii; ss.
+    { dependent destruction smos. ss. }
+    { dependent destruction smos. ss.
+      f_equal. eapply IHm; eauto.
+    }
+  Qed.
+
+  Lemma tmp_lemma_aux: forall `{SM: SimMem.class} {SS: SimSymb.class SM}
+              (msps: list ModSemPair.t)
+              n m msp
+              (LT: (n < m)%nat)
+              (MIDXFACT: forall o msp_o,
+                  nth_error msps o = Some msp_o ->
+                  msp_o.(ModSemPair.src).(midx) = o)
+              (MSP: nth_error msps n = Some msp),
+      (<<SMPROJ: forall smos (MWF: SimMem.wf (fst smos) /\
+                                   SimMemOhs_wf_aux msps (fst smos) m (snd smos)),
+          exists smo, sm_match_tmp_aux msps msp smo m (snd smos)
+                      /\ SimMemOh.sm smo = fst smos
+                      /\ SimMemOh.wf smo>>).
+  Proof.
+    ii.
+    destruct smos as [sm smos]; ss. des.
+    gen n.
+    dependent induction smos; ii; ss.
+    { omega. }
+    dependent destruction MWF0.
+    assert(LEN: length (rev (SimMemOhs_ohs_src_aux2 smos)) = n).
+    { rewrite rev_length. eapply ohs_src_aux2_length; eauto. }
+    destruct (classic (n0 = n)).
+    {
+      clarify.
+      exists hd. esplits; eauto.
+      - econs; ss.
+        + unfold SimMemOhs_ohs_src_aux. ss.
+          exploit (MIDXFACT n); eauto. intro T. rewrite T.
+          clear_tac.
+          rewrite nth_error_app2; cycle 1.
+          { omega. }
+          rewrite LEN. replace (n - n)%nat with 0%nat by omega.
+          ss.
+        + unfold SimMemOhs_ohs_src_aux. ss.
+          exploit (MIDXFACT n); eauto. intro T. rewrite T.
+          clear_tac.
+          rewrite nth_error_app2; cycle 1.
+          { omega. }
+          rewrite LEN. replace (n - n)%nat with 0%nat by omega.
+          ss.
+    }
+    exploit IHsmos; eauto.
+    { omega. }
+    i; des.
+    clarify.
+    exploit (MIDXFACT n0); eauto. intro T.
+    assert(LT2: (n0 < n)%nat) by omega.
+    esplits; eauto.
+    {
+      clear - LT2 T H0 LEN.
+      clear_tac.
+      inv H0.
+      econs; eauto.
+      - unfold SimMemOhs_ohs_src_aux in *. ss.
+        rewrite nth_error_app1; try omega. ss.
+      - unfold SimMemOhs_ohs_src_aux in *. ss.
+        rewrite nth_error_app1; try omega. ss.
+    }
+  Qed.
+
+  Goal forall `{SM: SimMem.class} {SS: SimSymb.class SM}
+              (msps: list ModSemPair.t)
+              n msp
+              (MSP: nth_error msps n = Some msp),
+      (<<SMPROJ: forall smos (MWF: SimMemOhs_wf msps smos),
+          exists smo, sm_match_tmp msps msp smo smos /\ SimMemOh.wf smo>>).
+  Proof.
+    ii. destruct smos as [sm smos]. rr in MWF. des.
+    exploit (@tmp_lemma_aux _ _ msps n (length msps)); eauto.
+    { eapply nth_error_Some; eauto. rewrite MSP; ss. }
+    { admit "". }
+    i; des. ss.
+    esplits; eauto. rr. esplits; eauto.
+  Qed.
+
+  TTTTTTTTTTTTTTTTTTTTTTTTTTTTTTTTTTTTTTTTTTTTTTTTTT
+
+  Goal forall `{SM: SimMem.class} {SS: SimSymb.class SM}
+              (msps: list ModSemPair.t)
+              n m msp
+              (LT: (m < n)%nat)
+              (MIDXFACT: forall o msp_o,
+                  nth_error msps o = Some msp_o ->
+                  msp_o.(ModSemPair.src).(midx) = o)
+              (MSP: nth_error msps n = Some msp),
+      (<<SMPROJ: forall smos (MWF: SimMem.wf (fst smos) /\
+                                   SimMemOhs_wf_aux msps (fst smos) m (snd smos)),
+          exists smo, sm_match_tmp_aux msps msp smo m (snd smos)
+                      /\ SimMemOh.sm smo = fst smos
+                      /\ SimMemOh.wf smo>>).
+  Proof.
+  Qed.
+
+  Goal forall `{SM: SimMem.class} {SS: SimSymb.class SM}
+              (msps: list ModSemPair.t)
+              n msp
+              (MSP: nth_error msps n = Some msp),
+      (<<SMPROJ: forall smos (MWF: SimMemOhs_wf msps smos),
+          exists smo, sm_match_tmp msps msp smo smos /\ SimMemOh.wf smo>>).
+  Proof.
+    ii.
+    gen n.
+    destruct smos as [sm smos].
+    dependent induction smos; ii; ss.
+    { destruct msps; ss. clarify. destruct n; ss. }
+    destruct msps; ss. clarify.
+    dependent destruction smos0.
+    simpl_depind. clarify. simpl_depind. clarify.
+    idtac "IHsmos-is-not well-formed".
+  Abort.
+
+  Goal forall `{SM: SimMem.class} {SS: SimSymb.class SM}
+              (msps: list ModSemPair.t)
+              n msp
+              (MSP: nth_error msps n = Some msp),
+      (<<SMPROJ: forall smos (MWF: SimMemOhs_wf msps smos),
+          exists smo, sm_match_tmp msps msp smo smos /\ SimMemOh.wf smo>>).
+  Proof.
+    (* Set Printing All. *)
+    intros ? ? ?.
+    ginduction msps; ii; ss.
+    { destruct n; ss. }
+    rename msp into mspA.
+    rr in smos. destruct smos as [smos0 smos1].
+    dependent destruction smos1.
+    rename msp into mspB.
+    Set Printing Implicit.
+    (* MSP0: mspB
+       hd: mspB
+       MWF: mspB
+
+       MSP: mspA
+       exists smo: mspA
+       SimMemOh.wf mspA
+     *)
+    destruct n; ss; clarify.
+    -
+      Set Printing Implicit.
+      exists hd.
+      admit "".
+    -
+      exploit IHmsps; eauto.
+      { Check ((smos0, smos1): SimMemOhs_t msps).
+        instantiate (1:= (smos0, smos1)).
+    i. assert(msps = []).
+    { destruct msps; ss. }
+    ii. clarify. ss.
+    generalize msps.
+    dependent destruction msps. hrewrite H.
+    destruct msps.
+    generalize msps.
+    Set Printing All.
+  Qed.
+
+  Goal forall n msp (MSP: nth_error msps n = Some msp),
+      (<<SMPROJ: forall smos (MWF: SimMemOhs_wf smos),
+          exists smo, sm_match_tmp msp smo smos /\ SimMemOh.wf smo>>).
+  Proof.
+    clear SimMemOhs_le.
+    (* Set Printing All. *)
+    intros ? ? ?.
+    generalize msp.
+    ii.
+    generalize smos.
+    Set Printing Implicit.
+    dependent destruction msps.
+    Set Printing All.
+    ii.
+    { Set Printing All.
+      generalize (@ModSemPair.SMO SM SS msp).
+      generalize (@ModSemPair.src SM SS msp). destruct msps.
+    ii.
+  Qed.
+
+  Goal forall m n msp (LT: (n < m)%nat) (MSP: nth_error msps n = Some msp),
+      (<<SMPROJ: forall sm (smos_aux: SimMemOhs_t_aux m)
+                        (MWF: SimMemOhs_wf_aux sm smos_aux),
+          exists (smo: SimMemOh.t),
+            sm = smo.(SimMemOh.sm) /\
+            (projT1 ((SimMemOhs_ohs_src_aux smos_aux)
+                       (msp.(ModSemPair.src).(midx)))) =
+             msp.(ModSemPair.src).(owned_heap) /\
+            (projT2 ((SimMemOhs_ohs_src_aux smos_aux)
+                       (msp.(ModSemPair.src).(midx)))
+                   ~= smo.(SimMemOh.oh_src)) /\
+            SimMemOh.wf smo>>).
+  Proof.
+    intro. induction m; ii; ss.
+    { inv MWF. simpl_depind. clarify. dependent destruction smos_aux.
+      omega. }
+    (* - destruct n; ss. *)
+    (*   { des_ifs. exists sm. esplits; eauto. } *)
+    - dependent destruction smos_aux.
+      rename msp into msp_n. rename msp0 into msp_m.
+      destruct n; ss; cycle 1.
+      { exploit (IHm n); eauto. { omega. }
+      }
+      { revert MSP0 MWF.
+        revert hd.
+        revert msp_m.
+        generalize (nth_error msps m = Some msp_m).
+        destruct msps. des_ifs. exists sm. esplits; eauto.
+        -
+      }
+  Qed.
+
+  Goal forall n msp (MSP: nth_error msps n = Some msp),
+      (<<SMPROJ: forall smos (MWF: SimMemOhs_wf smos),
+          exists smo, sm_match_tmp msp smo smos /\ SimMemOh.wf smo>>).
+  Proof.
+    clear SimMemOhs_le.
+    (* Set Printing All. *)
+    ii.
+    induction msps.
+    ii.
+    { Set Printing All.
+      generalize (@ModSemPair.SMO SM SS msp).
+      generalize (@ModSemPair.src SM SS msp). destruct msps.
+    ii.
+  Qed.
 
   Let SimMemOhs_le (smos0 smos1: SimMemOhs_t): Prop.
   Proof.
@@ -703,7 +1201,6 @@ Next Obligation.
   - eapply (SimMemOh.le X1 Y1).
   - eapply True.
 Defined.
-From Paco Require Import hpattern.
 Next Obligation.
   econs.
   - ii. r. des_ifs.
